Fix spec monoid

theories/os/spec.v
@@ -20,8 +20,43 @@ Inductive spec_code :=
 
 Inductive spec_step : spec_code → spec_state → spec_code → spec_state → Prop :=
 | spec_step_rel:
-    ∀ (r: spec_rel) s retv s',
-      r s retv s' → spec_step (SCrel r) s (SCdone retv) s'.
+    ∀ (r: spec_rel) s retv s' sf,
+      gset_dom sf ⊥ gset_dom s → r s retv s' →
+      spec_step (SCrel r) (sf ∪ s) (SCdone retv) (sf ∪ s').
+
+Lemma left_id_ss  (s' : spec_state):
+  ∅ ∪ s' = s'.
+Admitted.
+
+Lemma spec_step_rel' (r: spec_rel) s retv s':
+  r s retv s' → spec_step (SCrel r) s (SCdone retv) s'.
+Proof.
+  rewrite -{2}(left_id_ss s') -{2}(left_id_ss s).
+  intros. apply spec_step_rel=>//.
+Qed.
+
+Lemma union_assoc_disj (s1 s2 s: spec_state):
+  gset_dom s1 ⊥ gset_dom s2 → s1 ∪ (s2 ∪ s) = (s1 ∪ s2) ∪ s.
+Admitted.
+
+Lemma union_disj (sf sf0 s0: spec_state):
+  gset_dom sf ⊥ gset_dom (sf0 ∪ s0) → gset_dom sf ⊥ gset_dom sf0.
+Admitted.  
+
+Lemma foo (sf0 s0 sf: spec_state):
+  gset_dom sf0 ⊥ gset_dom s0 →
+  gset_dom sf ⊥ gset_dom (sf0 ∪ s0) →
+  gset_dom (sf ∪ sf0) ⊥ gset_dom s0.
+Admitted.
+
+Lemma spec_step_framing c c' sf s s':
+  gset_dom sf ⊥ gset_dom s → spec_step c s c' s' → spec_step c (sf ∪ s) c' (sf ∪ s').
+Proof.
+  inversion 2. subst.
+  rewrite union_assoc_disj=>//; last by eapply union_disj.
+  rewrite union_assoc_disj=>//; last by eapply union_disj.
+  by constructor; first by apply foo.
+Qed.
 
 (* Naive equivalence *)
 Instance spec_code_equiv: Equiv spec_code := (=).
@@ -53,11 +88,7 @@ Section rules.
     (∃ c0 s0 c s,
      own spec_gname (● (Some (to_agree (c : leibnizC spec_code)))) ∗
      own γ_sstate (● to_gen_heap s) ∗ ⌜ spec_step c0 s0 c s⌝)%I.
-
-  Lemma spec_step_framing c c' sf s s':
-    gset_dom sf ⊥ gset_dom s → spec_step c s c' s' → spec_step c (sf ∪ s) c' (sf ∪ s').
-  Admitted.
-
+    
   Lemma spec_step_trans c c' c'' s s' s'':
     spec_step c s c' s' → spec_step c' s' c'' s'' → spec_step c s c'' s''.
   Admitted.
